LabelFreeNoDia.v
@@ -1,4 +1,4 @@
-Add LoadPath "LabelFree/SingleUnbox/NoDiamond".
+Add LoadPath "LabelFree/NoDiamond".
 Require Export LFND_Shared LFND_Syntax LFND_Substitution
         LFND_PPermutLib LFND_EmptyEquivLib LFND_OkLib
         LFND_Semantics.
