LabeledNoDia.v
@@ -1,2 +1,0 @@
-Add LoadPath "Labeled/Lists/NoDiamond".
-Require Export LND_Shared LND_Syntax LND_OkLib LND_Substitution LND_Semantics.
